Cislo3.lean
@@ -1,15 +1,135 @@
 import Cislo1
 import Cislo2
---import Std.Data.List.Lemmas
+import Std.Data.Rat.Basic
+import Std.Data.Rat.Lemmas
+import Std.Data.List.Lemmas
+import Mathlib.Tactic.LibrarySearch
+import Mathlib.Tactic.Linarith
+import Mathlib.Data.Rat.Basic
+import Mathlib.Data.Real.Basic
+
+
+theorem konjunkce_komutativni_v1 {P Q : Prop} (predpoklad : P ∧ Q) : Q ∧ P := by
+  rcases predpoklad with ⟨p,q⟩
+  constructor
+  · exact q
+  · exact p
+
+theorem konjunkce_komutativni_v2 {P Q : Prop} : P ∧ Q → Q ∧ P := by
+  intro predpoklad
+  rcases predpoklad with ⟨p,q⟩
+  constructor
+  · exact q
+  · exact p
+
+theorem konjunkce_komutativni_v3 {P Q : Prop} : P ∧ Q → Q ∧ P := by
+  rintro ⟨p,q⟩
+  constructor
+  · exact q
+  · exact p
+
+theorem konjunkce_komutativni_v4 {P Q : Prop} : P ∧ Q → Q ∧ P := by
+  intro ⟨p,q⟩
+  exact ⟨q,p⟩
+
+theorem konjunkce_komutativni_v5 {P Q : Prop} : P ∧ Q → Q ∧ P := by
+  intro predpoklad
+  exact And.symm predpoklad
+
+theorem konjunkce_komutativni_v6 {P Q : Prop} : P ∧ Q → Q ∧ P := by
+  exact And.symm
+
+theorem konjunkce_komutativni_v7 {P Q : Prop} : P ∧ Q → Q ∧ P :=
+And.symm
+
+theorem konjunkce_komutativni_obousmerne {P Q : Prop} : P ∧ Q ↔ Q ∧ P := by
+  constructor
+  · intro ⟨p,q⟩
+    exact ⟨q,p⟩
+  · intro ⟨q,p⟩
+    exact ⟨p,q⟩
+
+theorem konjunkce_komutativni_obousmern {P Q : Prop} : P ∧ Q ↔ Q ∧ P := by
+  constructor
+  · intro predpoklad
+    exact konjunkce_komutativni_v1 predpoklad
+  · intro predpoklad
+    exact konjunkce_komutativni_v1 predpoklad
+
+theorem konjunkce_komutativni_obousmer {P Q : Prop} : P ∧ Q ↔ Q ∧ P := by
+  constructor
+  · apply konjunkce_komutativni_v7
+  · apply konjunkce_komutativni_v7
+
+theorem konjunkce_komutativni_rovnost {P Q : Prop} : (P ∧ Q) = (Q ∧ P) := by
+  rw [konjunkce_komutativni_obousmer]
+
 
 theorem krat_dva (n : Nat) : n * 2 = n + n := by
-  induction n
-  rfl
   rw [Nat.mul_succ, Nat.mul_one]
 
- theorem fibo_odpovida {m n : Nat} (platny : n < m) : List.get? (fibo_list m) n = some (fibonacci n) := by
-  induction n
-  unfold fibonacci
-  unfold fibo_list
+theorem krat_dva' : ∀ n : Nat, n * 2 = n + n := by
+  intro x
+  ring
+
+
+theorem cislo_55_je_fibonacciho : ∃ n : Nat, fibonacci n = 55 := by
+  use 10
+  rfl
+
+
+theorem tesne : ∀ n : Nat, ∃ m : Nat, ∀ k : Nat, (k ≤ n → k < m) ∧ (n < k → m ≤ k) := by
+  intro n
+  use n + 1
+  intro k
+  constructor
+  · intro k_le_n
+    rw [Nat.lt_succ]
+    exact k_le_n
+  · intro n_lt_k
+    rw [Nat.succ_le]
+    exact n_lt_k
+
+theorem tesne' : ∀ n : Nat, ∃ m : Nat, ∀ k : Nat, (k ≤ n → k < m) ∧ (n < k → m ≤ k) :=
+  fun n => ⟨n + 1, fun _ => ⟨Nat.lt_succ_of_le, Nat.succ_le.mpr⟩⟩
+
+
+theorem racionalni_cisla_jsou_husta (x z : ℚ) : x < z → ∃ y : ℚ, x < y ∧ y < z := by
+  intro mensi
+  use (x + z) / 2
+  constructor
+  · convert_to x / 2 + x / 2 < x / 2 + z / 2
+    · ring
+    · rw [add_div]
+    · apply add_lt_add_left
+      exact div_lt_div_of_lt two_pos mensi
+  · convert_to x / 2 + z / 2 < z / 2 + z / 2
+    · rw [add_div]
+    · ring
+    · apply add_lt_add_right
+      exact div_lt_div_of_lt two_pos mensi
+
+theorem realna_cisla_jsou_husta : ∀ x z : ℝ, x < z → ∃ y : ℝ, x < y ∧ y < z := by
+  intro x z mensi
+  use (x + z) / 2
+  constructor
+  · convert_to x / 2 + x / 2 < x / 2 + z / 2
+    · ring
+    · rw [add_div]
+    · apply add_lt_add_left
+      exact div_lt_div_of_lt two_pos mensi
+  · convert_to x / 2 + z / 2 < z / 2 + z / 2
+    · rw [add_div]
+    · ring
+    · apply add_lt_add_right
+      exact div_lt_div_of_lt two_pos mensi
+
+
+theorem obrat_obrat {α : Type} (l : List α) : obrat_rychle (obrat_rychle l) = l := by
   sorry
+
+theorem obrat_append {α : Type} (l₁ l₂ : List α) : obrat_rychle (l₁ ++ l₂) = obrat_rychle l₂ ++ obrat_rychle l₁ := by
   sorry
+
+theorem prilep_obrat_dela_palindrom {α : Type} [DecidableEq α] (l : List α) : palindrom (l ++ obrat_rychle l) := by
+  rw [palindrom, decide_eq_true_eq, obrat_append, obrat_obrat]
