lakefile.lean
@@ -10,6 +10,7 @@ lean_exe «lean-mam» {
 }
 
 require std from git "https://github.com/leanprover/std4" @ "main"
+require mathlib4 from git "https://github.com/leanprover-community/mathlib4" @ "master"
 
 lean_lib Cislo1
 lean_lib Cislo2
